\documentclass{article}
\usepackage{amsthm,amsmath}
\usepackage{amssymb}
\begin{document}
	\begin{flushleft}
		Estimate a least-squares regression.
	\[Y=X_{1}^{T}\tilde{\beta}_{1}+\tilde{\mu}\]
	Then regress the residuals on another set of regressors.
	\[\tilde{\mu}=X_{2}^{T}\tilde{\beta}_{2}+\tilde{e}\]
	Then regress on both set of regressors.
	\[Y=X_{1}^{T}\hat{\beta}_{1}+X_{2}^{T}\hat{\beta}_{2}+\hat{e}\]
	Is it true that $\tilde{\beta}_{2}=\hat{\beta}_{2}$?
	\end{flushleft}
	\begin{proof}
		~\\
		\linespread{1.5}
		$\tilde{\beta}_{2}=\hat{\beta}_{2}$ if and only if $X_{1}$ and $X_{2}$ are uncorrelated, i.e. $X_{1}^{T}X_{2}=0$\\
		Define $M_{i}=I-X_{i}(X_{i}^{T}X_{i})^{-1}X_{i}^{T}$\\
		We obtain $\tilde{\mu}=M_{1}Y$\\
		$\tilde{\beta}_{2}=(X_{2}^{T}X_{2})^{-1}X_{2}^{T}\tilde{\mu}=(X_{2}^{T}X_{2})^{-1}X_{2}^{T}M_{1}Y$\\
		$\hat{\beta}_{2}=(X_{2}^{T}M_{1}X_{2})^{-1}X_{2}^{T}M_{1}Y$\\
		Suppose $\tilde{\beta}_{2}=\hat{\beta}_{2}$, then
		\[(X_{2}^{T}X_{2})^{-1}X_{2}^{T}M_{1}Y=(X_{2}^{T}M_{1}X_{2})^{-1}X_{2}^{T}M_{1}Y\]
		By algebra, we obtain $X_{2}^{T}X_{2}=X_{2}^{T}M_{1}X_{2}$\\
		Thus,  \[X_{2}^{T}X_{2}=X_{2}^{T}(I-X_{1}(X_{1}^{T}X_{1})^{-1}X_{1}^{T})X_{2}\\
		=X_{2}^{T}X_{2}-X_{2}^{T}X_{1}(X_{1}^{T}X_{1})^{-1}X_{1}^{T}X_{2}\]
		Thus $X_{1}^{T}X_{2}=0$ since $(X_{1}^{T}X_{1})^{-1}$ is invertible. 
	\end{proof}
\end{document}